fix(proof-libs/fstar): `#a` instead of `a`

proof-libs/fstar-secret-integers/rust_primitives/Rust_primitives.Arrays.fst
@@ -8,7 +8,7 @@ let to_list (#t:Type) (s: t_Slice t): list t = Seq.seq_to_list s
 let to_of_list_lemma t l = Seq.lemma_list_seq_bij l
 let of_to_list_lemma t l = Seq.lemma_seq_list_bij l
 
-let map_array #n (arr: t_Array 'a n) (f: 'a -> 'b): t_Array 'b n 
+let map_array #a #b #n (arr: t_Array a n) (f: a -> b): t_Array b n 
   = FStar.Seq.map_seq_len f arr;
     FStar.Seq.map_seq f arr 
 
