proof-libs/fstar/rust_primitives/Rust_primitives.fst
@@ -4,12 +4,14 @@ include Rust_primitives.Integers
 include Rust_primitives.Arrays
 include Rust_primitives.BitVectors
 
-let (let?) (x: Core.Option.t_Option 'a) (f: 'a -> Core.Option.t_Option 'b): Core.Option.t_Option 'b
+let (let?) 
+  (#a #b: Type)
+  (x: Core.Option.t_Option a) (f: a -> Core.Option.t_Option b): Core.Option.t_Option b
   = match x with
   | Core.Option.Option_Some x -> f x
   | Core.Option.Option_None   -> Core.Option.Option_None
 
-let (let|) #e #a #b (x: Core.Result.t_Result a e) (f: a -> Core.Result.t_Result b e)
+let (let|) (#e #a #b: Type) (x: Core.Result.t_Result a e) (f: a -> Core.Result.t_Result b e)
     : Core.Result.t_Result b e
     = match x with
     | Core.Result.Result_Ok x -> f x
