proof-libs/fstar/core/Alloc.Slice.fst
@@ -2,4 +2,4 @@ module Alloc.Slice
 open Rust_primitives.Arrays
 open Alloc.Vec
 
-let impl__to_vec (s: t_Slice 'a): t_Vec 'a Alloc.Alloc.t_Global = s
+let impl__to_vec #a (s: t_Slice a): t_Vec a Alloc.Alloc.t_Global = s
