proof-libs/fstar/core/Core.Result.fst
@@ -3,7 +3,7 @@ module Core.Result
 type t_Result t e = | Result_Ok: v:t -> t_Result t e
                     | Result_Err of e
 
-let impl__unwrap (x: t_Result 't 'e {Result_Ok? x}): 't = Result_Ok?.v x
+let impl__unwrap #t #e (x: t_Result t e {Result_Ok? x}): t = Result_Ok?.v x
 let impl__map_err #e1 #e2 (x: t_Result 't e1) (f: e1 -> e2): t_Result 't e2
   = match x with
   | Result_Ok v -> Result_Ok v
